Add a naive implementation of the first compilation pass

Lib/Monads.v
@@ -1,21 +1,183 @@
+Require Import Coq.Lists.List.
+Require Import FunctionalExtensionality.
+
 Class Monad (M: Type -> Type) := {
   ret : forall {A}, A -> M A;
   bind : forall {A B}, M A -> (A -> M B) -> M B
 }.
 
-Instance option_monad : Monad option := {
-  ret A x := Some x;
-  bind A B x f :=
-    match x with
-    | Some y => f y
-    | None => None
-    end
+Hint Unfold ret.
+Hint Unfold bind.
+
+Class MonadLaws M `{Monad M} := {
+  m_left_identity :
+    forall A B (a: A) (f: A -> M B),
+      bind (ret a) f = f a;
+  m_right_identity :
+    forall A (m: M A),
+      bind m ret = m;
+  m_associativity :
+    forall A B C (m: M A) (f: A -> M B) (g: B -> M C),
+      bind (bind m f) g = bind m (fun x => bind (f x) g) 
 }.
 
+(** Option Monad **)
+
+Instance option_monad : Monad option := {
+ ret A x :=
+   Some x;
+ bind A B x f :=
+   match x with
+   | Some y => f y
+   | None => None
+   end
+}.
+
+Lemma option_monad_left_id:
+  forall A B (a: A) (f: A -> option B),
+    bind (ret a) f = f a.
+Proof.
+  auto.
+Qed.
+
+Lemma option_monad_right_id:
+  forall A (m: option A),
+    bind m ret = m.
+Proof.
+  intros.
+  destruct m; auto.
+Qed.
+
+Lemma option_monad_associativity:
+  forall A B C (m: option A) (f: A -> option B) (g: B -> option C),
+    bind (bind m f) g = bind m (fun x => bind (f x) g).
+Proof.
+  intros.
+  destruct m; auto.
+Qed.
+
+Instance option_monad_laws : MonadLaws option := {
+  m_left_identity := option_monad_left_id;
+  m_right_identity := option_monad_right_id;
+  m_associativity := option_monad_associativity
+}.
+
+(** State Monad **)
+
+Definition ST (S A: Type) := S -> A * S.
+
+Instance state_monad {S} : Monad (ST S) := {
+  ret A x :=
+    fun s => (x, s);
+  bind A B s f :=
+    fun x => let '(x', s') := s x in
+          (f x') s'
+}.
+
+Section StateMonad.
+  Variable S: Type.
+
+  Definition ST_get : ST S S :=
+    fun s => (s, s).
+
+  Definition ST_put (s: S) : ST S unit :=
+    fun _ => (tt, s).
+
+  Definition ST_modify (f: S -> S) : ST S unit :=
+    fun s => (tt, f s).
+
+  Definition ST_run {A} (m: ST S A) (s: S) : A * S :=
+    m s.
+
+  Lemma state_monad_left_id:
+    forall A B (a: A) (f: A -> ST S B),
+      bind (ret a) f = f a.
+  Proof.
+    auto.
+  Qed.
+
+  Lemma state_monad_right_id:
+    forall A (m: ST S A),
+      bind m ret = m.
+  Proof.
+    intros.
+    unfold ret, bind. simpl.
+    extensionality x.
+    destruct (m x); auto.
+  Qed.
+
+  Lemma state_monad_associativity:
+    forall A B C (m: ST S A) (f: A -> ST S B) (g: B -> ST S C),
+      bind (bind m f) g = bind m (fun x => bind (f x) g).
+  Proof.
+    intros.
+    unfold ret, bind. simpl.
+    extensionality x.
+    destruct m; auto.
+  Qed.
+End StateMonad.
+
+Instance state_monad_laws {S} : MonadLaws (ST S) := {
+  m_left_identity := state_monad_left_id S;
+  m_right_identity := state_monad_right_id S;
+  m_associativity := state_monad_associativity S
+}.
+
+(** List Monad **)
+
+Instance list_monad : Monad list := {
+  ret A x := x :: nil;
+  bind A B m f := concat (map f m)
+}.
+
+Lemma list_monad_left_id:
+  forall A B (x: A) (f: A -> list B),
+    bind (ret x) f = f x.
+Proof.
+  intros.
+  simpl. rewrite app_nil_r. reflexivity.
+Qed.
+
+Lemma list_monad_right_id:
+  forall A (m: list A),
+    bind m ret = m.
+Proof.
+  intros.
+  induction m; auto.
+  - simpl.
+    replace (a :: m) with (a :: bind m ret)
+      by (rewrite IHm; reflexivity).
+    reflexivity.
+Qed.
+
+Lemma list_monad_associativity:
+  forall A B C (m: list A) (f: A -> list B) (g: B -> list C),
+    bind (bind m f) g = bind m (fun x => bind (f x) g).
+Proof.
+  intros.
+  induction m; auto.
+  - simpl in *.
+    rewrite map_app, concat_app, IHm.
+    reflexivity.
+Qed.
+
+Instance list_monad_laws : MonadLaws list := {
+  m_left_identity := list_monad_left_id;
+  m_right_identity := list_monad_right_id;
+  m_associativity := list_monad_associativity
+}.
+
+(* Notations *)
+
 Module MonadNotations.
-  Notation "m >>= f" := (bind m f) (at level 60, right associativity).
-  Notation "' x <- m ; y " := (m >>= (fun x:_ => y))
-    (at level 65, x ident, only parsing, right associativity).
-  Notation "' ( x1 , x2 ) <- m ; y" := (m >>= (fun x => let '(x1,x2) := x in y))
-    (at level 65, x1 ident, x2 ident, only parsing, right associativity).
+
+Notation "'do' X <- A ; B" := (bind A (fun X:_ => B))
+  (at level 200, X ident, A at level 100, B at level 200)
+  : monad_scope.
+
+Notation "'do' ( X , Y ) <- A ; B" :=
+  (bind A (fun x:_ => let '(X,Y) := x in B))
+  (at level 200, X ident, A at level 100, B at level 200)
+  : monad_scope.
+
 End MonadNotations.
