S2I/CompMonad.v
@@ -1,0 +1,94 @@
+Require Import Common.Definitions.
+Require Import Common.Values.
+Require Export Lib.Monads.
+
+Require Import FunctionalExtensionality.
+
+(* the compilation monad *)
+
+Module Comp.
+  Section Def.
+    Variable env: Type.
+
+    Definition t (res: Type) := env -> option (res * env).
+
+    Definition ret A (x:A) := fun (s:env) => Some (x, s).
+
+    Definition bind A B (s: t A) (f: A -> t B) :=
+      fun x => match s x with
+            | Some (x',s') => (f x') s'
+            | None => None
+            end.
+
+    Definition get : t env :=
+      fun s => Some (s, s).
+
+    Definition put (s: env) : t unit :=
+      fun _ => Some (tt, s).
+
+    Definition modify (f: env -> env) : t unit :=
+      fun s => Some (tt, f s).
+
+    Definition lift {A} (x: option A) : t A :=
+      fun s => match x with
+            | None => None
+            | Some v => Some (v, s)
+            end.
+
+    Definition fail {A} : t A :=
+      fun _ => None.
+
+    Definition run {A} (s: env) (m: t A) : option A :=
+      match m s with
+      | None => None
+      | Some (v,s') => Some v
+      end.
+  End Def.
+End Comp.
+
+Instance compilation_monad {env} : Monad (Comp.t env) := {
+  ret := Comp.ret env;
+  bind := Comp.bind env
+}.
+
+Section CompMonadLaws.
+  Variable env: Type.
+  
+  Lemma comp_monad_left_id:
+    forall res1 res2 (e: res1) (f: res1 -> Comp.t env res2),
+      bind (ret e) f = f e.
+  Proof.
+    auto.
+  Qed.
+
+  Lemma comp_monad_right_id:
+    forall res (m: Comp.t env res),
+      bind m ret = m.
+  Proof.
+    intros.
+    unfold ret, bind. simpl.
+    unfold Comp.ret, Comp.bind.
+    extensionality x.
+    destruct (m x); auto.
+    destruct p. auto.
+  Qed.
+
+  Lemma comp_monad_associativity:
+    forall res1 res2 res3 (m: Comp.t env res1)
+      (f: res1 -> Comp.t env res2) (g: res2 -> Comp.t env res3),
+      bind (bind m f) g = bind m (fun x => bind (f x) g).
+  Proof.
+    intros.
+    unfold ret, bind. simpl.
+    unfold Comp.ret, Comp.bind.
+    extensionality x.
+    destruct m; auto.
+    destruct p. destruct (f r e); auto.
+  Qed.
+End CompMonadLaws.
+
+Instance comp_monad_laws {env} : MonadLaws (Comp.t env) := {
+  m_left_identity := comp_monad_left_id env;
+  m_right_identity := comp_monad_right_id env;
+  m_associativity := comp_monad_associativity env
+}.
