S2I/Compiler.v
@@ -1,0 +1,324 @@
+Require Import Common.Definitions.
+Require Import Source.Language.
+Require Import Intermediate.Machine.
+Require Import S2I.CompMonad.
+
+Import MonadNotations.
+Open Scope monad_scope.
+
+(* the compilation environment *)
+
+Record comp_env : Type := {
+  next_label: label;
+  current_component : Component.id;
+  local_buffers : NMap.t (list Block.id);
+  procs_labels : NMap.t (NMap.t label)
+}.
+
+(* easy environments updates *)
+
+Definition with_next_label l env :=
+  {| next_label := l;
+     current_component := current_component env;
+     local_buffers := local_buffers env;
+     procs_labels := procs_labels env |}.
+
+Definition with_current_component C env :=
+  {| next_label := next_label env;
+     current_component := C;
+     local_buffers := local_buffers env;
+     procs_labels := procs_labels env |}.
+
+Definition with_component_buffers C bufs env :=
+  {| next_label := next_label env;
+     current_component := current_component env;
+     local_buffers := NMap.add C bufs (local_buffers env);
+     procs_labels := procs_labels env |}.
+
+Definition with_new_proc_label C P l env :=
+  {| next_label := next_label env;
+     current_component := current_component env;
+     local_buffers := local_buffers env;
+     procs_labels :=
+       let proc_labels' :=
+           match NMap.find C (procs_labels env) with
+           | None => NMap.add P l (@NMap.empty label)
+           | Some labels => NMap.add P l labels
+           end
+       in NMap.add C proc_labels' (procs_labels env) |}.
+
+(* simplify notations *)
+
+Notation COMP := (Comp.t comp_env).
+Notation get := (Comp.get comp_env).
+Notation put := (Comp.put comp_env).
+Notation modify := (Comp.modify comp_env).
+Notation lift := (Comp.lift comp_env).
+Notation fail := (Comp.fail comp_env).
+Notation run := (Comp.run comp_env).
+
+(* auxiliary environment operations *)
+
+Definition fresh_label : COMP label :=
+  do cenv <- get;
+  let l := next_label cenv in
+  do _ <- modify (with_next_label (S l));
+  ret l.
+
+Definition get_local_buffer : COMP Pointer.t :=
+  do cenv <- get;
+  let C := current_component cenv in
+  do blocks <- lift (NMap.find C (local_buffers cenv));
+  do b <- lift (nth_error blocks 0);
+  ret (C, b, 0).
+
+Definition get_temp_buffer : COMP Pointer.t:=
+  do cenv <- get;
+  let C := current_component cenv in
+  do blocks <- lift (NMap.find C (local_buffers cenv));
+  do b <- lift (nth_error blocks (length blocks - 1));
+  ret (C, b, 0).
+
+Definition find_proc_label C P : COMP label :=
+  do cenv <- get;
+  do P_labels <- lift (NMap.find C (procs_labels cenv));
+  lift (NMap.find P P_labels).
+
+(* code generation *)
+
+Definition push (r: register) : code :=
+  [Store R_SP r;
+   BinOp Add R_SP R_ONE R_SP].
+
+Definition pop (r: register) : code :=
+  [BinOp Minus R_SP R_ONE R_SP;
+   Load R_SP r].
+
+Definition load_arg (buf: Pointer.t) (r: register) : code :=
+  [Const (IPtr buf) r;
+   Load r r].
+
+Definition store_arg (buf: Pointer.t) (r r': register) : code :=
+  [Const (IPtr buf) r';
+   Store r' r].
+
+Definition store_stack_frame_pointer (buf: Pointer.t) (r: register) : code :=
+  [Const (IPtr buf) r;
+   Store r R_SP].
+
+Definition restore_stack_frame_pointer (buf: Pointer.t) : code :=
+  [Const (IPtr buf) R_SP;
+   Load R_SP R_SP].
+
+Definition store_environment (buf: Pointer.t) : code :=
+  store_stack_frame_pointer buf R_AUX1.
+
+Definition restore_environment (buf: Pointer.t) : code :=
+  Const (IInt 1) R_ONE ::
+  restore_stack_frame_pointer buf.
+
+Fixpoint compile_expr (e: expr) : COMP code :=
+  match e with
+  | E_val (Int i) =>
+    ret [Const (IInt i) R_COM]
+  | E_val (Ptr p) =>
+    ret [Const (IPtr p) R_COM]
+  | E_val Undef => fail (* we don't compile undef *)
+  | E_local =>
+    do local_buf_ptr <- get_local_buffer;
+    ret [Const (IPtr local_buf_ptr) R_COM]
+  | E_binop bop e1 e2 =>
+    do c1 <- compile_expr e1;
+    do c2 <- compile_expr e2;
+    ret (c1 ++
+         push R_COM ++
+         c2 ++
+         pop R_AUX1 ++
+         BinOp bop R_AUX1 R_COM R_COM :: nil)
+  | E_seq e1 e2 =>
+    do c1 <- compile_expr e1;
+    do c2 <- compile_expr e2;
+    ret (c1 ++ c2)
+  | E_if e1 e2 e3 =>
+    do c1 <- compile_expr e1;
+    do c2 <- compile_expr e2;
+    do c3 <- compile_expr e3;
+    do lconseq <- fresh_label;
+    do lend <- fresh_label;
+    ret (c1 ++
+         [Bnz R_COM lconseq] ++
+         c3 ++
+         [Bnz R_ONE lend;
+          Label lconseq] ++
+         c2 ++
+         Label lend :: nil)
+  | E_alloc e =>
+    do c <- compile_expr e;
+    ret (c ++
+         Alloc R_COM R_COM :: nil)
+  | E_deref e =>
+    do c <- compile_expr e;
+    ret (c ++
+         Load R_COM R_COM :: nil)
+  | E_assign e1 e2 =>
+    do c1 <- compile_expr e1;
+    do c2 <- compile_expr e2;
+    ret (c1 ++
+         push R_COM ++
+         c2 ++
+         pop R_AUX1 ++
+         Store R_COM R_AUX1 :: nil)
+  | E_call C' P' e =>
+    do cenv <- get;
+    let C := current_component cenv in
+    do local_buf_ptr <- get_local_buffer;
+    do call_arg_code <- compile_expr e;
+    if C' =? C then
+      do target_label <- find_proc_label C' P';
+      ret (call_arg_code ++
+           push R_AUX2 ++
+           load_arg local_buf_ptr R_AUX1 ++
+           push R_AUX1 ++
+           [Jal target_label] ++
+           pop R_AUX1 ++
+           store_arg local_buf_ptr R_AUX1 R_AUX2 ++
+           pop R_AUX2)
+    else
+      do temp_buf_ptr <- get_temp_buffer;
+      ret (call_arg_code ++
+           push R_AUX2 ++
+           load_arg local_buf_ptr R_AUX1 ++
+           push R_AUX1 ++
+           store_environment temp_buf_ptr ++
+           [Call C' P'] ++
+           restore_environment temp_buf_ptr ++
+           pop R_AUX1 ++
+           store_arg local_buf_ptr R_AUX1 R_AUX2 ++
+           pop R_AUX2)
+  | E_exit => ret [Halt]
+  end.
+
+Definition compile_proc
+           (C: Component.id) (P: Procedure.id) (e: expr)
+  : COMP code :=
+  do _ <- modify (with_current_component C);
+  do proc_label <- find_proc_label C P;
+  do local_buf_ptr <- get_local_buffer;
+  do lmain <- fresh_label;
+  do lreturn <- fresh_label;
+  do proc_code <- compile_expr e;
+  (* TODO compute stack size *)
+  let stack_frame_size := 100 in
+  ret ([Const (IInt 1) R_ONE;
+        Const (IInt 1) R_AUX2;
+        Const (IInt stack_frame_size) R_SP;
+       Alloc R_SP R_SP;
+       Bnz R_ONE lmain;
+       Label proc_label;
+       Const (IInt 0) R_AUX2;
+       Mov R_SP R_AUX1;
+       Const (IInt stack_frame_size) R_SP;
+       Alloc R_SP R_SP] ++
+       push R_AUX1 ++
+       [Label lmain] ++
+       push R_RA ++
+       store_arg local_buf_ptr R_COM R_AUX1 ++
+       proc_code ++
+       pop R_RA ++
+       [Bnz R_AUX2 lreturn] ++
+       pop R_SP ++
+       [Jump R_RA;
+        Label lreturn;
+        Return]).
+
+Fixpoint gen_component_procedures_labels
+         (C: Component.id) (procs: list (Procedure.id * expr))
+  : COMP unit :=
+  match procs with
+  | [] => ret tt
+  | (P, _) :: procs' =>
+    do freshl <- fresh_label;
+    do _ <- modify (with_new_proc_label C P freshl);
+    gen_component_procedures_labels C procs'
+  end.
+
+(* think about labels collision when linking partial programs *)
+Fixpoint gen_all_procedures_labels
+         (procs: list (Component.id * NMap.t expr))
+  : COMP unit :=
+  match procs with
+  | [] => ret tt
+  | (C, Cprocs) :: procs' =>
+    do _ <- gen_component_procedures_labels C (NMap.elements Cprocs);
+    gen_all_procedures_labels procs'
+  end.
+
+Fixpoint add_temporary_buffers
+         (bufs: list (Component.id * nat))
+  : COMP (NMap.t (list (Block.id * nat))) :=
+  let fix instrument acc bs :=
+      match bs with
+      | [] => ret acc
+      | (C,size) :: bs' =>
+        let Cbufs := [(0,size); (1,1)] in
+        let acc' := NMap.add C Cbufs acc in
+        do _ <- modify (with_component_buffers C (map fst Cbufs));
+        instrument acc' bs'
+      end
+  in instrument (NMap.empty (list (Block.id * nat))) bufs.
+
+Fixpoint compile_procedures
+         (C: Component.id)
+         (procs: list (Procedure.id * expr))
+  : COMP (list (Procedure.id * code)) :=
+  let fix compile acc ps :=
+      match ps with
+      | [] => ret acc
+      | (P,e) :: ps' =>
+        do proc_code <- compile_proc C P e;
+        let acc' := (P,proc_code) :: acc in
+        compile acc' ps'
+      end
+  in compile [] procs.
+
+Fixpoint compile_components
+         (comps: list (Component.id * NMap.t expr))
+  : COMP (list (Component.id * NMap.t code)) :=
+  let fix compile acc cs :=
+      match cs with
+      | [] => ret acc
+      | (C,procs) :: cs' =>
+        do procs_code <- compile_procedures C (NMap.elements procs);
+        let acc' := (C, NMapExtra.of_list procs_code) :: acc in
+        compile acc' cs'
+      end
+  in compile [] comps.
+
+Definition init_env : comp_env :=
+  {| next_label := 0;
+     current_component := 0;
+     local_buffers := @NMap.empty (list Block.id);
+     procs_labels := @NMap.empty (NMap.t label) |}.
+
+Definition compile_program
+           (p: Source.program) : option Intermediate.program :=
+  let procs := NMap.elements (Source.prog_procedures p) in
+  let bufs := NMap.elements (Source.prog_buffers p) in
+  run init_env (
+    do _ <- gen_all_procedures_labels procs;
+    do bufs' <- add_temporary_buffers bufs;
+    do code <- compile_components procs;
+    ret {| Intermediate.prog_interface := Source.prog_interface p;
+           Intermediate.prog_procedures := NMapExtra.of_list code;
+           Intermediate.prog_buffers := bufs' |}).
+
+(*
+Require Import Source.Examples.
+
+Eval compute in run init_env
+                    (compile_expr (E_binop Add
+                                           (E_val (Int 41))
+                                           (E_val (Int 1)))).
+
+Eval compute in compile_program factorial.
+*)
