Source/Examples.v
@@ -1,0 +1,28 @@
+Require Import Common.Definitions.
+Require Import Common.Values.
+Require Import Source.Language.
+Require Import Source.CS.
+Require Import Lib.Tactics.
+Require Import CompCert.Smallstep.
+Require Import CompCert.Events.
+
+Import Source.
+
+(* naive factorial *)
+
+Definition factorial : program := {|
+  prog_interface :=
+    NMapExtra.of_list [(1, {| Component.import := [(2, 0)];
+                              Component.export := [1] |});
+                       (2, {| Component.import := [];
+                              Component.export := [1] |})];
+  prog_buffers := NMapExtra.of_list [(1, 1); (2, 1)];
+  prog_procedures := NMapExtra.of_list [
+    (1, NMapExtra.of_list [(0, E_call 2 0 (E_val (Int 3)))]);
+    (2, NMapExtra.of_list [(0,
+      E_if (E_binop Leq (E_deref E_local) (E_val (Int 1)))
+        (E_val (Int 1))
+        (E_binop Mul
+                 (E_deref E_local)
+                 (E_call 2 0 (E_binop Minus (E_deref E_local) (E_val (Int 1))))))])]
+|}.
